Example.v
@@ -67,3 +67,83 @@ Defined.
 (*
 Eval compute in (proj1_sig rev3_exists').
 *)
+
+(* examples for PRO-99 *)
+
+Set Printing Width 51.
+
+Lemma example1 a b c d :
+  ([:: a; b; c; d], [::
+   instswap; instpop; instswap; instquote; instquote;
+   instcopy; instcons; instswap; instquote; instquote;
+   instcons; instexec; instswap; instcons; instquote;
+   instcons; instswap; instquote; instcons; instexec;
+   instquote; instcons; instexec]) |=>*
+  ([:: d; c; a; c], [::]).
+Proof.
+  eapply evalrtc_cons.
+  Show Existentials.
+  by apply evalswap.
+  do !econstructor.
+  Undo.
+  set cs := [:: instexec];
+    move: {1 3}cs (eq_refl cs); subst cs => cs Hcs.
+  do !econstructor.
+  Undo.
+  evalauto.
+  rewrite Hcs.
+  evalauto.
+Qed.
+
+Lemma example2 :
+  { p | forall a b c d,
+    ([:: a; b; c; d], p) |=>*
+    ([:: d; c; a; c], [::]) }.
+Proof.
+  eexists => a b c d.
+  eapply evalrtc_cons; first by apply evalswap.
+  evalpartial evalpop. evalpartial evalswap.
+  evalpartial evalquote. evalpartial evalquote.
+  evalpartial evalcopy. evalpartial evalcons.
+  evalpartial evalswap. evalpartial evalquote.
+  evalpartial evalquote. evalpartial evalcons.
+  evalpartial evalexec. evalauto.
+  evalpartial evalswap. evalpartial evalcons.
+  evalpartial evalquote. evalpartial evalcons.
+  evalpartial evalswap. evalpartial evalquote.
+  evalpartial evalcons. evalpartial evalexec.
+  evalauto.
+  evalpartial evalquote. evalpartial evalcons.
+  evalpartial evalexec. evalauto.
+Defined.
+
+Goal forall a, a = size [::tt; tt] -> a = 2.
+Proof.
+  move=> a H.
+  (eapply eq_trans; first apply H); simpl.
+  Undo.
+  (eapply eq_trans; first apply H);
+    subst_evars; simpl.
+  done.
+Qed.
+
+Eval compute in (proj1_sig example2).
+
+Lemma example3 :
+  { p |
+    forall i1 i2 i3 vs cs,
+    (i1 :: i2 :: i3 :: vs, p :: cs) |=>*
+    (instpair i1 instsnoc ::
+     instpair i3 (instpush i1) :: vs, cs) }.
+Proof.
+  eexists => i1 i2 i3 vs cs.
+  evaltemplate 3
+    [:: insttpair (instthole 0)
+          (instt_of_inst instsnoc);
+        insttpair (instthole 2)
+          (insttpush (instthole 0))]
+    (Nil instt).
+  evalauto.
+Defined.
+
+Eval compute in (inst_size (proj1_sig example3)).
