embed.m4
@@ -1,9 +1,6 @@
 define(`EMBED',
     `syscmd(./coq2ps -m "MODULES" "$1" | tr -d "\n")dnl'
 )dnl
-define(`EMBEDPUSH',
-    `{EMBED($1)}dnl'
-)dnl
 define(`SET_MODULES',
     `define(`MODULES', `$1')dnl'
 )dnl
